\tasknumber{2018}{4} Решить уравнение: $(x^2-2x)^2-2x^2+4x=3$.

\Solution Выделим в левой части полный квадрат:
\begin{center}
$(x^2-2x)^2-2x^2+4x=3 \Leftrightarrow(x^2-2x)^2-2(x^2-2x)\hm=3 \Leftrightarrow (x^2-2x)^2-2(x^2-2x)+1\hm=4 \hm \Leftrightarrow (x^2-2x-1)^2\hm=4 \hm\Leftrightarrow \left[
\begin{array}{l}
x^2-2x-1=2,\\
x^2-2x-1=-2
\end{array} 
\right. \hm\Leftrightarrow \left[
\begin{array}{l}
x^2-2x-3=0,\\
x^2-2x+1=0
\end{array} 
\right.\hm \Leftrightarrow \left[
\begin{array}{l}
(x-3)(x+1)=0,\\
(x-1)^2=0
\end{array} 
\right.\hm \Leftrightarrow \left[
\begin{array}{l}
x=3,\\
x=-1,\\
x=1.
\end{array} 
\right. $ 
\end{center}

\Answer{$\{-1;1;3\}$}
